src/Std/Data/HashSet/RawLemmas.lean
@@ -817,15 +817,14 @@ theorem isEmpty_of_isEmpty_insertMany [EquivBEq α] [LawfulHashable α] (h : m.W
 section
 variable {m₁ m₂ : Raw α}
 
-theorem Equiv.beq [LawfulHashable α] [EquivBEq α] (h₁ : m₁.WF) (h₂ : m₂.WF) : m₁ ~m m₂ → beq m₁ m₂ := fun hyp =>
-  @HashMap.Raw.Equiv.beq _ _ _ _ m₁.1 m₂.1 _ _ _ _ h₁.1 h₂.1 hyp.1
+theorem Equiv.beq [LawfulHashable α] [EquivBEq α] (h₁ : m₁.WF) (h₂ : m₂.WF) : m₁ ~m m₂ → beq m₁ m₂ :=
+  fun hyp => HashMap.Raw.Equiv.beq h₁.1 h₂.1 hyp.1
 
-theorem equiv_of_beq [LawfulBEq α] (h₁ : m₁.WF) (h₂ : m₂.WF) : m₁ == m₂ → m₁ ~m m₂ := fun hyp =>
-  ⟨@HashMap.Raw.equiv_of_beq _ _ _ _ m₁.1 m₂.1 _ _ _ h₁.1 h₂.1 hyp⟩
+theorem equiv_of_beq [LawfulBEq α] (h₁ : m₁.WF) (h₂ : m₂.WF) : m₁ == m₂ → m₁ ~m m₂ :=
+  fun hyp => ⟨HashMap.Raw.equiv_of_beq h₁.1 h₂.1 hyp⟩
 
-theorem Equiv.beq_congr [EquivBEq α] [LawfulHashable α] {m₃ m₄ : Raw α} (h₁ : m₁.WF) (h₂ : m₂.WF) (h₃ : m₃.WF) (h₄ : m₄.WF)  :
-    m₁ ~m m₃ → m₂ ~m m₄ → (m₁ == m₂) = (m₃ == m₄) := fun hyp1 hyp2 =>
-  @HashMap.Raw.Equiv.beq_congr _ _ _ _ m₁.1 m₂.1 _ _ _ m₃.1 m₄.1 h₁.1 h₂.1 h₃.1 h₄.1 hyp1.1 hyp2.1
+theorem Equiv.beq_congr [EquivBEq α] [LawfulHashable α] {m₃ m₄ : Raw α} (h₁ : m₁.WF) (h₂ : m₂.WF) (h₃ : m₃.WF) (h₄ : m₄.WF) : m₁ ~m m₃ → m₂ ~m m₄ → (m₁ == m₂) = (m₃ == m₄) :=
+  fun hyp1 hyp2 => HashMap.Raw.Equiv.beq_congr h₁.1 h₂.1 h₃.1 h₄.1 hyp1.1 hyp2.1
 
 end
 
